src/temporal_logic/persistent.lean
@@ -7,9 +7,10 @@ variables {α : Sort u₀} {β : Type u₁} {γ : Sort u₂}
 
 namespace temporal
 open predicate
-class persistent (p : cpred) : Prop :=
-  (is_persistent : ◻p = p)
-export persistent (is_persistent)
+
+class postponable (p : cpred) : Prop :=
+  (postpone : ◇p = p)
+export postponable (postpone)
 
 instance henceforth_persistent {p : cpred} : persistent (◻p) :=
 by { constructor, simp }
@@ -27,10 +28,6 @@ by { constructor, simp [henceforth_and,is_persistent], }
 instance coe_persistent (p : Prop)
 : persistent (p : cpred) :=
 by { constructor, cases classical.prop_complete p ; subst p ; simp, }
-
-instance true_persistent
-: persistent (True : cpred) :=
-by { constructor, simp, }
 
 instance false_persistent
 : persistent (False : cpred) :=
@@ -55,19 +52,14 @@ instance not_forall_persistent {p : α → cpred} [∀ i, persistent (- p i)]
 : persistent (- p_forall p) :=
 by { constructor, simp [p_not_p_forall], apply is_persistent }
 
-def list_persistent (xs : list cpred) :=
-Π q ∈ xs, persistent q
+inductive list_persistent : list cpred → Prop
+ | nil_persistent : list_persistent []
+ | cons_persistent (x : cpred) (xs : list $ cpred)
+   [persistent x]
+   (h : list_persistent xs)
+ : list_persistent (x :: xs)
 
-lemma nil_persistent
-: list_persistent [] :=
-by { intros p h, cases h }
-
-lemma cons_persistent (x : cpred) (xs : list $ cpred)
-  [persistent x]
-  (h : list_persistent xs)
-: list_persistent (x :: xs) :=
-by { intros p h, simp [list_persistent] at *,
-     cases h ; [ subst p, skip ] ; auto, }
+export list_persistent (nil_persistent)
 
 def with_h_asms (Γ : cpred) : Π (xs : list (cpred)) (x : cpred), Prop
  | [] x := Γ ⊢ x
@@ -84,32 +76,11 @@ lemma judgement_trans (p q r : pred' β)
 : p ⊢ r :=
 sorry
 
-lemma from_antecendent (xs : list (cpred)) (p : cpred)
-  (h : ∀ Γ, with_h_asms Γ xs p)
-: ◻ xs.foldr (⋀) True ⊢ p :=
-begin
-  apply indirect_judgement,
-  introv h', specialize h Γ,
-  induction xs with x xs,
-  { simp [with_h_asms] at h, apply h },
-  { simp [list.foldr,henceforth_and] at h',
-    apply xs_ih,
-    { revert h',
-      apply p_impl_revert,
-      apply p_and_elim_right },
-    { apply h, revert h',
-      apply p_impl_revert,
-      apply p_and_entails_of_entails_left,
-      apply henceforth_str, } }
-end
-
-class postponable (p : cpred) : Prop :=
-  (postpone : ◇p = p)
-export postponable (postpone)
-
-lemma p_imp_postpone (Γ p q : cpred) [postponable q]
-  (h : tl_imp Γ p q)
-: tl_imp Γ (◇p) q :=
+lemma p_imp_postpone (Γ p q : cpred)
+  [persistent Γ]
+  [postponable q]
+  (h : ctx_impl Γ p q)
+: ctx_impl Γ (◇p) q :=
 begin
   rw ← postpone q,
   monotonicity h,
@@ -136,8 +107,9 @@ instance exists_postponable (p : α → cpred) [∀ i, postponable (p i)]
 by constructor ; simp [eventually_exists,postpone]
 
 lemma persistent_to_henceforth {p q : cpred}
-  (h : ◻ p ⊢ q)
-: ◻ p ⊢ ◻ q :=
+  [persistent p]
+  (h : p ⊢ q)
+: p ⊢ ◻ q :=
 sorry
 
 lemma henceforth_deduction {Γ p q : cpred}
